DynamoDbEncryption/runtimes/java/src/main/smithy-generated/software/amazon/cryptography/dynamoDbEncryption/itemEncryptor/ToDafny.java
@@ -52,34 +52,6 @@ public class ToDafny {
     return Error.create_CollectionOfErrors(list);
   }
 
-  public static DecryptItemInput DecryptItemInput(
-      software.amazon.cryptography.dynamoDbEncryption.itemEncryptor.model.DecryptItemInput nativeValue) {
-    DafnyMap<? extends DafnySequence<? extends Character>, ? extends AttributeValue> encryptedItem;
-    encryptedItem = Dafny.Com.Amazonaws.Dynamodb.ToDafny.AttributeMap(nativeValue.encryptedItem());
-    return new DecryptItemInput(encryptedItem);
-  }
-
-  public static DecryptItemOutput DecryptItemOutput(
-      software.amazon.cryptography.dynamoDbEncryption.itemEncryptor.model.DecryptItemOutput nativeValue) {
-    DafnyMap<? extends DafnySequence<? extends Character>, ? extends AttributeValue> plaintextItem;
-    plaintextItem = Dafny.Com.Amazonaws.Dynamodb.ToDafny.AttributeMap(nativeValue.plaintextItem());
-    return new DecryptItemOutput(plaintextItem);
-  }
-
-  public static EncryptItemOutput EncryptItemOutput(
-      software.amazon.cryptography.dynamoDbEncryption.itemEncryptor.model.EncryptItemOutput nativeValue) {
-    DafnyMap<? extends DafnySequence<? extends Character>, ? extends AttributeValue> encryptedItem;
-    encryptedItem = Dafny.Com.Amazonaws.Dynamodb.ToDafny.AttributeMap(nativeValue.encryptedItem());
-    return new EncryptItemOutput(encryptedItem);
-  }
-
-  public static EncryptItemInput EncryptItemInput(
-      software.amazon.cryptography.dynamoDbEncryption.itemEncryptor.model.EncryptItemInput nativeValue) {
-    DafnyMap<? extends DafnySequence<? extends Character>, ? extends AttributeValue> plaintextItem;
-    plaintextItem = Dafny.Com.Amazonaws.Dynamodb.ToDafny.AttributeMap(nativeValue.plaintextItem());
-    return new EncryptItemInput(plaintextItem);
-  }
-
   public static DynamoDbItemEncryptorConfig DynamoDbItemEncryptorConfig(
       software.amazon.cryptography.dynamoDbEncryption.itemEncryptor.model.DynamoDbItemEncryptorConfig nativeValue) {
     DafnySequence<? extends Character> tableName;
@@ -117,6 +89,34 @@ public class ToDafny {
         Option.create_Some(software.amazon.cryptography.dynamoDbEncryption.ToDafny.LegacyConfig(nativeValue.legacyConfig()))
         : Option.create_None();
     return new DynamoDbItemEncryptorConfig(tableName, partitionKeyName, sortKeyName, attributeActions, allowedUnauthenticatedAttributes, allowedUnauthenticatedAttributePrefix, algorithmSuiteId, keyring, cmm, legacyConfig);
+  }
+
+  public static DecryptItemInput DecryptItemInput(
+      software.amazon.cryptography.dynamoDbEncryption.itemEncryptor.model.DecryptItemInput nativeValue) {
+    DafnyMap<? extends DafnySequence<? extends Character>, ? extends AttributeValue> encryptedItem;
+    encryptedItem = Dafny.Com.Amazonaws.Dynamodb.ToDafny.AttributeMap(nativeValue.encryptedItem());
+    return new DecryptItemInput(encryptedItem);
+  }
+
+  public static EncryptItemInput EncryptItemInput(
+      software.amazon.cryptography.dynamoDbEncryption.itemEncryptor.model.EncryptItemInput nativeValue) {
+    DafnyMap<? extends DafnySequence<? extends Character>, ? extends AttributeValue> plaintextItem;
+    plaintextItem = Dafny.Com.Amazonaws.Dynamodb.ToDafny.AttributeMap(nativeValue.plaintextItem());
+    return new EncryptItemInput(plaintextItem);
+  }
+
+  public static DecryptItemOutput DecryptItemOutput(
+      software.amazon.cryptography.dynamoDbEncryption.itemEncryptor.model.DecryptItemOutput nativeValue) {
+    DafnyMap<? extends DafnySequence<? extends Character>, ? extends AttributeValue> plaintextItem;
+    plaintextItem = Dafny.Com.Amazonaws.Dynamodb.ToDafny.AttributeMap(nativeValue.plaintextItem());
+    return new DecryptItemOutput(plaintextItem);
+  }
+
+  public static EncryptItemOutput EncryptItemOutput(
+      software.amazon.cryptography.dynamoDbEncryption.itemEncryptor.model.EncryptItemOutput nativeValue) {
+    DafnyMap<? extends DafnySequence<? extends Character>, ? extends AttributeValue> encryptedItem;
+    encryptedItem = Dafny.Com.Amazonaws.Dynamodb.ToDafny.AttributeMap(nativeValue.encryptedItem());
+    return new EncryptItemOutput(encryptedItem);
   }
 
   public static Error Error(DynamoDbItemEncryptorException nativeValue) {
