DynamoDbEncryption/dafny/DynamoDbEncryption/Model/AwsCryptographyDynamoDbEncryptionTypes.dfy
@@ -25,14 +25,9 @@ include "../../../../submodules/MaterialProviders/StandardLibrary/src/Index.dfy"
  predicate method IsValid_BeaconBitLength(x: int32) {
  ( 1 <= x <= 63 )
 }
- datatype BeaconKey = | BeaconKey (
- nameonly keyArn: string ,
- nameonly tableArn: string ,
- nameonly branchKeyID: string
- )
  datatype BeaconVersion = | BeaconVersion (
  nameonly version: VersionNumber ,
- nameonly key: BeaconKey ,
+ nameonly keyring: AwsCryptographyMaterialProvidersTypes.IKeyring ,
  nameonly standardBeacons: Option<StandardBeaconList> ,
  nameonly compoundBeacons: Option<CompoundBeaconList> ,
  nameonly virtualFields: Option<VirtualFieldList>
