DynamoDbEncryption/dafny/DynamoDbEncryption/src/Beacon.dfy
@@ -3,7 +3,7 @@
 
 include "Util.dfy"
 include "Virtual.dfy"
-include "DynamoToStruct.dfy"
+include "../../../../submodules/MaterialProviders/StandardLibrary/src/HexStrings.dfy"
 
 module BaseBeacon {
   import opened Wrappers
@@ -14,7 +14,6 @@ module BaseBeacon {
   import opened HexStrings
   import opened DynamoDbEncryptionUtil
   import opened DdbVirtualFields
-  import DynamoToStruct
 
   import DDB = ComAmazonawsDynamodbTypes
   import Prim = AwsCryptographyPrimitivesTypes
@@ -149,21 +148,23 @@ module BaseBeacon {
       var bytes :- VirtToBytes(loc, item, vf);
       hash(bytes)
     }
-
-    function method GetFields(virtualFields : VirtualFieldMap) : seq<string>
+    
+/*
+    function method {:opaque} getHash(byteify : Byteify)
+      : (ret : Result<string, Error>)
+      ensures ret.Success? ==>
+        && |ret.value| > 0
     {
-      if loc[0].key in virtualFields then
-        virtualFields[loc[0].key].GetFields()
-      else
-        [loc[0].key]
+      var bytes :- byteify(loc).MapFailure(e => E(e));
+      hash(bytes)
+    }
+*/
+    // TODO virtual fields
+    function method GetFields() : seq<string>
+    {
+      [loc[0].key]
     }
 
-    function method GetBeaconValue(value : DDB.AttributeValue) : Result<DDB.AttributeValue, Error>
-    {
-      var bytes :- DynamoToStruct.TopLevelAttributeToBytes(value).MapFailure(e => E(e));
-      var h :- hash(bytes);
-      Success(DDB.AttributeValue.S(h))
-    }
 
     //= specification/searchable-encryption/beacons.md#getpart-for-a-standard-beacon
     //= type=implication
@@ -184,9 +185,6 @@ module BaseBeacon {
     {
         base.hash(val, length)
     }
-
-    function method ValidStateResult() : Result<bool, Error> {Success(true)}
-    predicate method ValidState() {true}
   }
 
   // For a given BeaconLength, how many chars in the associated hex string?
