DynamoDbEncryption/dafny/DynamoDbEncryption/test/Virtual.dfy
@@ -2,7 +2,6 @@
 // SPDX-License-Identifier: Apache-2.0
 
 include "../src/UpdateExpr.dfy"
-include "../src/Virtual.dfy"
 
 module TestDdbVirtualFields {
 
