DynamoDbEncryption/dafny/DynamoDbEncryptionTransforms/src/DdbMiddlewareConfig.dfy
@@ -1,6 +1,7 @@
 // Copyright Amazon.com Inc. or its affiliates. All Rights Reserved.
 // SPDX-License-Identifier: Apache-2.0
 include "../Model/AwsCryptographyDynamoDbEncryptionTransformsTypes.dfy"
+include "DynamoDbMiddlewareSupport.dfy"
 
 module DdbMiddlewareConfig {
   import opened Wrappers
