DynamoDbEncryption/dafny/DynamoDbEncryptionTransforms/src/ScanTransform.dfy
@@ -1,7 +1,7 @@
 // Copyright Amazon.com Inc. or its affiliates. All Rights Reserved.
 // SPDX-License-Identifier: Apache-2.0
 
-include "DynamoDbMiddlewareSupport.dfy"
+include "DdbMiddlewareConfig.dfy"
 
 module ScanTransform {
   import opened DdbMiddlewareConfig
@@ -65,7 +65,9 @@ module ScanTransform {
       && output.value.transformedOutput == input.sdkOutput
 
     ensures output.Success?  && input.sdkOutput.Items.None?  ==> output.value.transformedOutput.Items.None?
-    ensures output.Success?  && input.sdkOutput.Items.Some?  ==> output.value.transformedOutput.Items.Some?
+    ensures output.Success?  && input.sdkOutput.Items.Some?  ==>
+      && output.value.transformedOutput.Items.Some?
+      && |output.value.transformedOutput.Items.value| == |input.sdkOutput.Items.value|
 
     ensures output.Success? && input.sdkOutput.Items.Some? && input.originalInput.TableName in config.tableEncryptionConfigs ==>
       var oldHistory := old(config.tableEncryptionConfigs[input.originalInput.TableName].itemEncryptor.History.DecryptItem);
