DynamoDbEncryption/dafny/DynamoDbEncryptionTransforms/test/ExecuteTransactionTransform.dfy
@@ -1,7 +1,7 @@
 // Copyright Amazon.com Inc. or its affiliates. All Rights Reserved.
 // SPDX-License-Identifier: Apache-2.0
-include "../src/Index.dfy"
-include "TestFixtures.dfy"
+include "../../DynamoDbEncryptionTransforms/src/Index.dfy"
+include "../../DynamoDbEncryption/test/TestFixtures.dfy"
 
 module ExecuteTransactionTransformTest {
   import opened Wrappers
